share/steel/examples/steel/dplex/out/EffectSystemProperties.ml
@@ -1,0 +1,18 @@
+open Prims
+let pending (es : EffectStateMachine.effect_state) :
+  Domain.action Prims.list=
+  (es.EffectStateMachine.client).MultiCollaboration.pending
+let pending_tail (es : EffectStateMachine.effect_state) :
+  Domain.action Prims.list=
+  match pending es with | [] -> [] | uu___::tl -> tl
+let rec apply_events (next : Prims.nat -> Prims.nat)
+  (es : EffectStateMachine.effect_state)
+  (events : EffectStateMachine.event Prims.list) :
+  EffectStateMachine.effect_state=
+  match events with
+  | [] -> es
+  | ev::tl ->
+      let uu___ = EffectStateMachine.step next es ev in
+      (match uu___ with | (es1, _cmd) -> apply_events next es1 tl)
+type ('es, 'ev, 'a) processed_now = Obj.t
+type ('next, 'es, 'events, 'a) action_was_processed = Obj.t
