share/steel/examples/steel/dplex/out/PingPongTest.ml
@@ -1,55 +1,47 @@
 open Prims
-let (pingpong : Steel_Channel_Duplex.prot) =
+let pingpong : Steel_Channel_Duplex.prot=
   Steel_Channel_Protocol.bind (Steel_Channel_Protocol.send ())
     (fun x ->
        Steel_Channel_Protocol.bind (Steel_Channel_Protocol.recv ())
          (fun y -> Steel_Channel_Protocol.done1))
-let (client : Obj.t Steel_Channel_Duplex.chan -> unit) =
-  fun c ->
-    Steel_Channel_Duplex.send pingpong c pingpong
-      (Obj.magic (Prims.of_int (17)));
-    (let y =
-       Steel_Channel_Duplex.recv pingpong
-         (Steel_Channel_Protocol.step pingpong
-            (Obj.magic (Prims.of_int (17)))) c in
-     ())
-let (server : Obj.t Steel_Channel_Duplex.chan -> unit) =
-  fun c ->
-    let y =
-      Steel_Channel_Duplex.recv pingpong
-        (Steel_Channel_Protocol.dual pingpong) c in
-    Steel_Channel_Duplex.send pingpong c
-      (Steel_Channel_Protocol.step (Steel_Channel_Protocol.dual pingpong) y)
-      (Obj.magic ((Obj.magic y) + (Prims.of_int (42))))
-let (client_server : unit -> unit) =
-  fun uu___ ->
-    let c = Steel_Channel_Duplex.new_chan pingpong in
-    let uu___1 =
-      Steel_Effect.par () () (fun uu___2 -> client c) () ()
-        (fun uu___2 -> server c) in
-    ()
-let rec (join_all : unit Steel_Primitive_ForkJoin.thread Prims.list -> unit)
-  =
-  fun threads ->
-    if FStar_List_Tot_Base.isEmpty threads
-    then ()
-    else
-      (let uu___1 = threads in
-       match uu___1 with
-       | hd::tl ->
-           (Steel_Primitive_ForkJoin.join () (Obj.magic hd); join_all tl))
-let rec (many :
-  Prims.nat -> unit Steel_Primitive_ForkJoin.thread Prims.list -> unit) =
-  fun n ->
-    fun threads ->
-      if n = Prims.int_zero
-      then join_all threads
-      else
-        Steel_Primitive_ForkJoin.fork () () () () client_server
-          (fun uu___2 ->
-             fun uu___1 ->
-               (fun t ->
-                  let t = Obj.magic t in
-                  fun uu___1 ->
-                    Obj.magic (many (n - Prims.int_one) (t :: threads)))
-                 uu___2 uu___1)
+let client (c : Obj.t Steel_Channel_Duplex.chan) : unit=
+  Steel_Channel_Duplex.send pingpong c pingpong
+    (Obj.magic (Prims.of_int (17)));
+  (let y =
+     Steel_Channel_Duplex.recv pingpong
+       (Steel_Channel_Protocol.step pingpong (Obj.magic (Prims.of_int (17))))
+       c in
+   ())
+let server (c : Obj.t Steel_Channel_Duplex.chan) : unit=
+  let y =
+    Steel_Channel_Duplex.recv pingpong (Steel_Channel_Protocol.dual pingpong)
+      c in
+  Steel_Channel_Duplex.send pingpong c
+    (Steel_Channel_Protocol.step (Steel_Channel_Protocol.dual pingpong) y)
+    (Obj.magic ((Obj.magic y) + (Prims.of_int (42))))
+let client_server (uu___ : unit) : unit=
+  let c = Steel_Channel_Duplex.new_chan pingpong in
+  let uu___1 =
+    Steel_Effect.par () () (fun uu___2 -> client c) () ()
+      (fun uu___2 -> server c) in
+  ()
+let rec join_all (threads : unit Steel_Primitive_ForkJoin.thread Prims.list)
+  : unit=
+  if FStar_List_Tot_Base.isEmpty threads
+  then ()
+  else
+    (let uu___1 = threads in
+     match uu___1 with
+     | hd::tl ->
+         (Steel_Primitive_ForkJoin.join () (Obj.magic hd); join_all tl))
+let rec many (n : Prims.nat)
+  (threads : unit Steel_Primitive_ForkJoin.thread Prims.list) : unit=
+  if n = Prims.int_zero
+  then join_all threads
+  else
+    Steel_Primitive_ForkJoin.fork () () () () client_server
+      (fun uu___2 uu___1 ->
+         (fun t ->
+            let t = Obj.magic t in
+            fun uu___1 -> Obj.magic (many (n - Prims.int_one) (t :: threads)))
+           uu___2 uu___1)
